src/Var.v
@@ -10,26 +10,35 @@ Import Prenex Implicits.
 
 
 
+Delimit Scope var_scope with var.
+
+(* Typed variables *)
+
 Section Var.
 
-  Record var : Set := mkVar { vname :> N; vtyp : typ }.
+  Local Open Scope var_scope.
+
+  Record var : Set := mkVar { vname : N; vtyp : typ; vidx : N }.
 
   Definition vsize v := sizeof_typ (vtyp v).
 
-  Definition var_eqn (x y : var) : bool := (vname x == vname y) && (vtyp x == vtyp y).
+  (* Strong equality *)
+
+  Definition var_eqn (x y : var) : bool :=
+    (vname x == vname y) && (vtyp x == vtyp y) && (vidx x == vidx y).
+
+  Notation "x =? y" := (var_eqn x y) : var_scope.
 
   Lemma var_eqn_eq (x y : var) : x = y <-> var_eqn x y.
   Proof.
     destruct x; destruct y; split; rewrite /var_eqn /=.
-    - move=> [] -> ->. by rewrite !eqxx.
-    - move/andP => [/eqP -> /eqP ->]. reflexivity.
+    - move=> [] -> -> ->. by rewrite !eqxx.
+    - move=> /andP [/andP [/eqP -> /eqP ->] /eqP ->]. reflexivity.
   Qed.
 
-  Notation "x =? y" := (var_eqn x y).
-
-  Lemma var_eqP : forall (x y : var), reflect (x = y) (x =? y).
+  Lemma var_eqP : forall (x y : var), reflect (x = y) (var_eqn x y).
   Proof.
-    move=> x y. case H: (x =? y).
+    move=> x y. case H: (var_eqn x y).
     - apply: ReflectT. apply/var_eqn_eq. assumption.
     - apply: ReflectF. move=> Heq. move/var_eqn_eq: Heq => Heq. rewrite Heq in H.
       discriminate.
@@ -39,32 +48,41 @@ Section Var.
   Canonical var_eqType := Eval hnf in EqType var var_eqMixin.
 
   Lemma var_eqn_vname (x y : var) : x == y -> vname x = vname y.
-  Proof. destruct x; destruct y => /=. move/eqP=> H. by case: H. Qed.
+  Proof. by move=> /andP [/andP [/eqP -> _] _]. Qed.
 
   Lemma var_eqn_vtyp (x y : var) : x == y -> vtyp x = vtyp y.
-  Proof. destruct x; destruct y => /=. move/eqP=> H. by case: H. Qed.
+  Proof. by move=> /andP [/andP [_ /eqP ->] _]. Qed.
 
-  Lemma var_neq_case (x y : var) : x != y = (vname x != vname y) || (vtyp x != vtyp y).
+  Lemma var_eqn_vidx (x y : var) : x == y -> vidx x = vidx y.
+  Proof. by move=> /andP [/andP [_ _] /eqP ->]. Qed.
+
+  Lemma var_neq_case (x y : var) :
+    x != y = (vname x != vname y) || (vtyp x != vtyp y) || (vidx x != vidx y).
   Proof.
-    destruct x; destruct y => /=. case H: ((vname0 != vname1) || (vtyp0 != vtyp1)).
-    - case/orP: H.
-      + move=> H. apply/negP => /eqP [] Hn Ht. rewrite Hn eqxx in H. discriminate.
-      + move=> H. apply/negP => /eqP [] Hn Ht. rewrite Ht eqxx in H. discriminate.
-    - move: (Bool.orb_false_elim _ _ H) => {H} [/negPn Hn /negPn Ht].
-      apply/negPn/eqP. by rewrite (eqP Hn) (eqP Ht); reflexivity.
+    destruct x; destruct y => /=.
+    case H: ((vname0 != vname1) || (vtyp0 != vtyp1) || (vidx0 != vidx1)).
+    - case/orP: H; first case/orP.
+      + move=> H. apply/negP => /eqP [] Hn Ht Hi. rewrite Hn eqxx in H. discriminate.
+      + move=> H. apply/negP => /eqP [] Hn Ht Hi. rewrite Ht eqxx in H. discriminate.
+      + move=> H. apply/negP => /eqP [] Hn Ht Hi. rewrite Hi eqxx in H. discriminate.
+    - move: (Bool.orb_false_elim _ _ H) => {H} [H /negPn Hi].
+      move: (Bool.orb_false_elim _ _ H) => {H} [/negPn Hn /negPn Ht].
+      apply/negPn/eqP. by rewrite (eqP Hn) (eqP Ht) (eqP Hi); reflexivity.
   Qed.
 
   Definition var_ltn (x y : var) : bool :=
-    (vname x <? vname y)%num || (vname x == vname y) && (vtyp x <? vtyp y)%typ.
+    (vname x <? vname y)%num
+    || (vname x == vname y) && (vtyp x <? vtyp y)%typ
+    || (vname x == vname y) && (vtyp x == vtyp y)%typ && (vidx x <? vidx y)%num.
 
   Notation "x <? y" := (var_ltn x y).
 
   Lemma var_ltnn (x : var) : (x <? x) = false.
   Proof.
-    destruct x; rewrite /var_ltn /=. rewrite Nltnn eqxx typ_ltnn. reflexivity.
+    destruct x; rewrite /var_ltn /=. rewrite !Nltnn !eqxx typ_ltnn. reflexivity.
   Qed.
 
-  Lemma var_ltn_eqF (x y : var) : x <? y -> x == y = false.
+  Lemma var_ltn_eqF (x y : var) : x <? y -> (x == y) = false.
   Proof.
     move=> Hlt. apply/negP=> /eqP Heq. rewrite Heq var_ltnn in Hlt. discriminate.
   Qed.
@@ -72,31 +90,45 @@ Section Var.
   Lemma var_ltn_trans (x y z : var) : x <? y -> y <? z -> x <? z.
   Proof.
     destruct x; destruct y; destruct z; rewrite /var_ltn => /=. move=> Hxy Hyz.
-    case/orP: Hxy; case/orP: Hyz.
+    case/orP: Hxy; first case/orP; case/orP: Hyz; first case/orP.
     - move=> Hn12 Hn01. by rewrite (Nltn_trans Hn01 Hn12).
     - move/andP=> [Hn12 Ht12] Hn01. rewrite (eqP Hn12) in Hn01. by rewrite Hn01.
-    - move=> Hn12 /andP [Hn01 Ht01]. by rewrite (eqP Hn01) Hn12.
-    - move=> /andP [Hn12 Ht12] /andP [Hn01 Ht01]. rewrite (eqP Hn01) (eqP Hn12) eqxx.
-      rewrite (typ_ltn_trans Ht01 Ht12). by rewrite orbT.
+    - move=> /andP [/andP [Hn12 Ht12] Hv12] Hv01. rewrite (eqP Hn12) in Hv01.
+      by rewrite Hv01.
+    - move=> Hn12 /andP [Hn01 Ht01]. case/orP: Hn12.
+      + move=> Hn12. by rewrite (eqP Hn01) Hn12.
+      + move/andP=> [Hn12 Ht12]. rewrite (eqP Hn01) (eqP Hn12) eqxx.
+        by rewrite (typ_ltn_trans Ht01 Ht12) orbT.
+    - move=> /andP [/andP [Hn12 Ht12] Hi12] /andP [Hn01 Ht01].
+      rewrite (eqP Hn01) (eqP Hn12) eqxx. rewrite (eqP Ht12) in Ht01.
+      by rewrite Ht01 orbT.
+    - case/orP; [move=> Hn12 | move=> /andP [Hn12 Ht12]];
+        move=> /andP [/andP [Hn01 Ht01] Hi01].
+      + by rewrite (eqP Hn01) Hn12.
+      + by rewrite (eqP Hn01) (eqP Hn12) eqxx (eqP Ht01) Ht12 orbT.
+    - move=> /andP [/andP [Hn12 Ht12] Hi12] /andP [/andP [Hn01 Ht01] Hi01].
+        by rewrite (eqP Hn01) (eqP Hn12) (eqP Ht01) (eqP Ht12) !eqxx
+                   (Nltn_trans Hi01 Hi12) orbT.
   Qed.
 
   Lemma var_ltn_neqAlt (x y : var) : x <? y = (x != y) && ~~ (y <? x).
   Proof.
     destruct x; destruct y; rewrite /var_ltn => /=. rewrite var_neq_case /=.
     rewrite negb_or negb_and. rewrite (eq_sym vname1 vname0).
-    case Hneq01: (vname0 == vname1) => /=.
-    - rewrite (eqP Hneq01) => {Hneq01}. rewrite Nltnn /=. exact: typ_ltn_neqAlt.
-    - rewrite orbF andbT. rewrite Nltn_neqAlt. move/idP/negP: Hneq01 => ->.
-      reflexivity.
+    case Hnne01: (vname0 == vname1) => /=.
+    - rewrite (eqP Hnne01) => {Hnne01}. rewrite Nltnn /=.
+      rewrite (eq_sym vtyp1 vtyp0). case Htne01: (vtyp0 == vtyp1) => /=.
+      + rewrite (eqP Htne01) => {Htne01}. rewrite typ_ltnn /=. exact: Nltn_neqAlt.
+      + rewrite typ_ltn_neqAlt orbF. move/idP/negP: Htne01 => ->. by rewrite andbT.
+    - rewrite !orbF andbT. rewrite Nltn_neqAlt. by move/idP/negP: Hnne01 => ->.
   Qed.
 
   Lemma var_neq_ltn (x y : var) : (x != y) = (x <? y) || (y <? x).
   Proof.
     case Heq: (x == y).
     - rewrite (eqP Heq) var_ltnn. reflexivity.
-    - case Hlt: (x <? y).
-      + reflexivity.
-      + symmetry => /=. rewrite var_ltn_neqAlt eq_sym Heq Hlt. reflexivity.
+    - case Hlt: (x <? y) => //=.
+      symmetry. by rewrite var_ltn_neqAlt eq_sym Heq Hlt.
   Qed.
 
   Definition var_compare (x y : var) : Compare var_ltn eq_op x y.
@@ -109,22 +141,117 @@ Section Var.
 
 End Var.
 
+Notation "x =? y" := (var_eqn x y) : var_scope.
+Notation "x <? y" := (var_ltn x y) : var_scope.
+
 Module VarOrderedMinimal : SsrOrderedTypeMinimal.
   Definition t := var_eqType.
-  Definition eq (x y : t) := x == y.
-  Definition lt := var_ltn.
-  Definition lt_trans := var_ltn_trans.
-  Lemma lt_not_eq (x y : t) : lt x y -> x != y.
+  Definition eqn (x y : t) := x == y.
+  Definition ltn := var_ltn.
+  Definition ltn_trans := var_ltn_trans.
+  Lemma ltn_not_eqn (x y : t) : ltn x y -> x != y.
   Proof. move=> H. rewrite (var_ltn_eqF H). done. Qed.
   Definition compare := var_compare.
 End VarOrderedMinimal.
+Module VarOrder <: SsrOrderedTypeWithFacts := MakeSsrOrderedType VarOrderedMinimal.
 
-Module VarOrder := MakeSsrOrderedType VarOrderedMinimal.
+Module VS := MakeTreeSet VarOrder.
+Module VM := MakeTreeMap VarOrder.
 
-Module VS := MakeTreeSet NOrder.
-Module VM := MakeTreeMap NOrder.
 
-Delimit Scope var_scope with var.
 
-Notation "x =? y" := (var_eqn x y) : var_scope.
-Notation "x <? y" := (var_ltn x y) : var_scope.
+(* Untyped variables *)
+
+Definition var_untyped v := (vname v, vidx v).
+
+Coercion var_untyped : var >-> prod.
+
+Module UVarOrder <: SsrOrderedTypeWithFacts := MakeProdOrdered NOrder NOrder.
+
+Module UVS := MakeTreeSet UVarOrder.
+Module UVM := MakeTreeMap UVarOrder.
+
+Section UntypedVar.
+
+  Local Open Scope var_scope.
+
+  (* Weak equality *)
+
+  Definition uvar_eqn (x y : var) : bool := var_untyped x == var_untyped y.
+
+  Infix "=??" := uvar_eqn (at level 70) : var_scope.
+
+  Notation "x !=?? y" := (~~ (uvar_eqn x y)) (at level 70, no associativity) : var_scope.
+
+  Lemma uvar_eqn_case (x y : var) :
+    (x =?? y) = (vname x == vname y) && (vidx x == vidx y).
+  Proof.
+    case: x => nx tx ix; case: y => ny ty iy /=. case H: ((nx == ny) && (ix == iy)).
+    - move/andP: H=> [/eqP -> /eqP ->]. exact: eqxx.
+    - case: (Bool.andb_false_elim _ _ H) => {H} H.
+      + apply/negP => /eqP [] Hn Hi; subst. by rewrite eqxx in H.
+      + apply/negP => /eqP [] Hn Hi; subst. by rewrite eqxx in H.
+  Qed.
+
+  Lemma uvar_eqn_vname (x y : var) : x =?? y -> vname x = vname y.
+  Proof. by rewrite uvar_eqn_case => /andP [/eqP -> _]. Qed.
+
+  Lemma uvar_eqn_vidx x y : x =?? y -> vidx x = vidx y.
+  Proof. by rewrite uvar_eqn_case => /andP [_ /eqP ->]. Qed.
+
+  Lemma uvar_neq_case (x y : var) :
+    x !=?? y = (vname x != vname y) || (vidx x != vidx y).
+  Proof. by rewrite uvar_eqn_case negb_and. Qed.
+
+  Lemma uvar_eqn_refl (x : var) : x =?? x.
+  Proof. exact: eqxx. Qed.
+
+  Lemma uvar_eqn_sym (x y : var) : (x =?? y) = (y =?? x).
+  Proof. by rewrite /uvar_eqn eq_sym. Qed.
+
+  Lemma uvar_eqn_symmetric (x y : var) : (x =?? y) -> (y =?? x).
+  Proof. by rewrite uvar_eqn_sym. Qed.
+
+  Lemma uvar_eqn_trans (x y z : var) : x =?? y -> y =?? z -> x =?? z.
+  Proof. move=> /eqP H1 /eqP H2. by rewrite /uvar_eqn H1 H2. Qed.
+
+  Global Instance uvar_eqn_Reflexive : Reflexive (@uvar_eqn) := @uvar_eqn_refl.
+  Global Instance uvar_eqn_Symmetric : Symmetric (@uvar_eqn) := @uvar_eqn_symmetric.
+  Global Instance uvar_eqn_Transitive : Transitive (@uvar_eqn) := @uvar_eqn_trans.
+  Instance uvar_eqn_Equivalence : Equivalence uvar_eqn :=
+    { Equivalence_Reflexive := uvar_eqn_Reflexive;
+      Equivalence_Symmetric := uvar_eqn_Symmetric;
+      Equivalence_Transitive := uvar_eqn_Transitive }.
+
+  Definition uvar_ltn (x y : var) : bool := UVarOrder.ltn x y.
+
+  Infix "<??" := uvar_ltn (at level 70) : var_scope.
+
+  Lemma uvar_ltnn (x : var) : (x <?? x) = false.
+  Proof. exact: UVarOrder.ltnn. Qed.
+
+  Lemma uvar_ltn_weqF (x y : var) : x <?? y -> x =?? y = false.
+  Proof. exact: UVarOrder.ltn_eqF. Qed.
+
+  Lemma uvar_ltn_trans (x y z : var) : x <?? y -> y <?? z -> x <?? z.
+  Proof. exact: UVarOrder.ltn_trans. Qed.
+
+  Lemma uvar_ltn_wneqAlt (x y : var) : x <?? y = (x !=?? y) && ~~ (y <?? x).
+  Proof. exact: UVarOrder.ltn_neqAlt. Qed.
+
+  Lemma uvar_neq_wltn (x y : var) : (x !=?? y) = (x <?? y) || (y <?? x).
+  Proof. exact: UVarOrder.neq_ltn. Qed.
+
+  Definition uvar_compare (x y : var) : Compare uvar_ltn uvar_eqn x y.
+  Proof.
+    case: (UVarOrder.compare x y) => H.
+    - apply: LT. exact: H.
+    - apply: EQ. exact: H.
+    - apply: GT. exact: H.
+  Defined.
+
+End UntypedVar.
+
+Infix "=??" := uvar_eqn (at level 70) : var_scope.
+Notation "x !=?? y" := (~~ (uvar_eqn x y)) (at level 70, no associativity) : var_scope.
+Infix "<??" := uvar_ltn (at level 70) : var_scope.
